LeanYjs/Transitivity.lean
@@ -1,0 +1,52 @@
+import LeanYjs.Item
+import LeanYjs.ActorId
+import LeanYjs.ItemOriginOrder
+import LeanYjs.ItemOrder
+import LeanYjs.ItemSet
+import LeanYjs.ItemSetInvariant
+
+variable {A : Type} {P : ClosedPredicate A} {inv : ItemSetInvariant P}
+
+lemma yjs_lt_item (x : YjsItem A) (y : YjsPtr A) :
+  YjsLt P h x y -> (∃ y', y = YjsPtr.itemPtr y') ∨ y = YjsPtr.last := by
+  intros hlt
+  revert x y
+  apply Nat.strongRecOn' (P := fun h => ∀ (x : YjsItem A) (y : YjsPtr A), YjsLt P h (YjsPtr.itemPtr x) y → (∃ y', y = YjsPtr.itemPtr y') ∨ y = YjsPtr.last) h
+  intros n ih x y hlt
+  cases hlt with
+  | ltConflict h x y hlt =>
+    cases hlt with
+    | ltOriginDiff h1 h2 h3 h4 l1 l2 r1 r2 id1 id2 c1 c2 hlt1 hlt2 hlt3 =>
+      left; constructor; eq_refl
+    | ltOriginSame h1 h2 l r1 r2 id1 id2 c1 c2 hlt1 hlt2 _ =>
+      left; constructor; eq_refl
+  | ltOriginOrder x y hpx hpy hlt =>
+    cases hlt with
+    | lt_left o r id c =>
+      left; constructor; eq_refl
+    | lt_right o r id c
+
+
+
+
+lemma yjs_lt_transitivity {A : Type} {P : ClosedPredicate A} {inv : ItemSetInvariant P} :
+  ∀ (x y z : YjsPtr A), P.val x -> P.val y -> P.val z ->
+  YjsLt' P x y -> YjsLt' P y z -> YjsLt' P x z := by
+  intros x y z hx hy hz hxy hyz
+  unfold YjsLt' at *
+  obtain ⟨ P, hP ⟩ := P
+  obtain ⟨ h0, hxy ⟩ := hxy
+  obtain ⟨ h1, hyz ⟩ := hyz
+  generalize hsize : x.size + y.size + z.size = total_size
+  revert x y z
+  simp
+  apply @Nat.strongRecOn' (P := fun ts => ∀ x y z,
+    P x → P y → P z →
+    YjsLt ⟨ P, hP ⟩ h0 x y → YjsLt ⟨ P, hP ⟩ h1 y z → x.size + y.size + z.size = ts → ∃ h, YjsLt ⟨P, hP⟩ h x z) total_size
+  intros total_size ih x y z hx hy hz hxy hyz hsize
+  cases hxy with
+  | ltOriginOrder _ _ hpx hpy hxy =>
+    simp at *
+    cases hxy with
+    | lt_left o r id c =>
+      simp [YjsPtr.size, YjsItem.size] at hsize
